WIP

src/make_ruletable.lean
@@ -1,5 +1,7 @@
 import data.finmap
 import .hitchhike
+import order.lexicographic
+import data.equiv.list
 
 inductive vonNeumann
   | N
@@ -7,84 +9,91 @@ inductive vonNeumann
   | S
   | W
 
-def vonNeumann.to_fin4 : vonNeumann → fin 4
+open vonNeumann
 
-def vonNeumann_fin4 : vonNeumann ≃ fin 4 :=
-  { to_fun := _,
-  inv_fun := _,
-  left_inv := _,
-  right_inv := _ }
-
-def vonNeumann.cmp (x y : vonNeumann) : ordering :=
-  match x, y with
-  | vonNeumann.N, vonNeumann.N := ordering.eq
-  | vonNeumann.N, _ := ordering.lt
-  | vonNeumann.E, vonNeumann.N := ordering.gt
-  | vonNeumann.E, vonNeumann.E := ordering.eq
-  | vonNeumann.E, _ := ordering.lt
-  | vonNeumann.S, vonNeumann.S := ordering.eq
-  | vonNeumann.S, vonNeumann.W := ordering.lt
-  | vonNeumann.S, _ := ordering.gt
-  | vonNeumann.W, vonNeumann.W := ordering.eq
-  | vonNeumann.W, _ := ordering.gt
+def vonNeumann.to_fin4 (dir : vonNeumann) : fin 4 :=
+  match dir with
+  | N := 0
+  | E := 1
+  | S := 2
+  | W := 3
   end
 
-lemma list.mem_pair {α} {x y z : α} {p : Prop} : x ∈ [y, z] → (x = y → p) → (x = z → p) → p :=
-  by {
-    intros x_y_z x_y x_z, 
-    cases x_y_z, 
-    apply x_y x_y_z, 
-    cases x_y_z, 
-    apply x_z x_y_z,
-    cases x_y_z,
-  }
+def fin.to_vonNeumann  : fin 4 → vonNeumann
+  | ⟨0, _⟩ := N
+  | ⟨1, _⟩ := E 
+  | ⟨2, _⟩ := S
+  | ⟨3, _⟩ := W
+  | ⟨n+4, p⟩ := false.rec vonNeumann (not_le.mpr p ((4 : ℕ).le_add_left n))
 
-instance : preorder vonNeumann := 
-  {
-    le := λ x y, x.cmp y ∈ [ordering.eq, ordering.lt],
-    le_refl := by {intros, unfold has_le.le, cases a; left; unfold vonNeumann.cmp},
-    le_trans := 
-    by {
-      intros a b c, 
-      unfold has_le.le, 
-      intros a_b b_c,
-      apply list.mem_pair a_b; clear a_b; intros a_b,
-      {
-        cases a; cases b; cases a_b; exact b_c,
-      },
-      right; left,
-      apply list.mem_pair b_c; clear b_c; intros b_c,
-      {
-        cases b; cases c; cases b_c; exact a_b,
-      },
-      cases a; cases b; cases a_b; cases c; cases b_c; trivial,
-    }
-  }
+lemma vonNeumann.aux (x : fin 4) : x.to_vonNeumann.to_fin4 = x :=
+  match x with
+  | ⟨0, _⟩ := rfl
+  | ⟨1, _⟩ := rfl 
+  | ⟨2, _⟩ := rfl
+  | ⟨3, _⟩ := rfl
+  | ⟨n+4, p⟩ := false.rec _ (not_le.mpr p ((4 : ℕ).le_add_left n))
+  end
 
-
-lemma vonNeumann_linear_order_aux (a b : vonNeumann) : (a.cmp b).compares a b := 
-  by {
-    cases a; cases b; unfold vonNeumann.cmp; unfold ordering.compares; 
-    unfold has_lt.lt gt; unfold_projs; unfold vonNeumann.cmp,
-    all_goals {
-      split,
-      {right, left, refl},
-      intros h, cases h; cases h; cases h,
-    },
-  }
-
-instance : linear_order vonNeumann := 
-  linear_order_of_compares vonNeumann.cmp vonNeumann_linear_order_aux
+def vonNeumann_fin4 : vonNeumann ≃ fin 4 :=
+{ 
+  to_fun := vonNeumann.to_fin4,
+  inv_fun := fin.to_vonNeumann,
+  left_inv := λ x, by {cases x; unfold vonNeumann.to_fin4; refl},
+  right_inv := λ x, by {apply vonNeumann.aux}
+}
 
 inductive Moore
-  | N
+  | NN
   | NE
-  | E
+  | EE
   | SE
-  | S
+  | SS
   | SW
-  | W
+  | WW
   | NW
+
+  open Moore
+
+def Moore.to_fin8 : Moore → fin 8 
+| NN := 0
+| NE := 1
+| EE := 2
+| SE := 3
+| SS := 4
+| SW := 5
+| WW := 6
+| NW := 7
+
+def fin.toMoore : fin 8 → Moore 
+  | ⟨0, _⟩ := NN
+  | ⟨1, _⟩ := NE 
+  | ⟨2, _⟩ := EE 
+  | ⟨3, _⟩ := SE 
+  | ⟨4, _⟩ := SS 
+  | ⟨5, _⟩ := SW 
+  | ⟨6, _⟩ := WW 
+  | ⟨7, _⟩ := NW
+  | ⟨n+8, p⟩ := false.rec _ (not_le.mpr p ((8 : ℕ).le_add_left n))
+
+def fin.toMoore.aux : ∀ x : fin 8, x.toMoore.to_fin8 = x 
+  | ⟨0, _⟩ := rfl
+  | ⟨1, _⟩ := rfl
+  | ⟨2, _⟩ := rfl
+  | ⟨3, _⟩ := rfl
+  | ⟨4, _⟩ := rfl
+  | ⟨5, _⟩ := rfl
+  | ⟨6, _⟩ := rfl
+  | ⟨7, _⟩ := rfl
+  | ⟨n+8, p⟩ := false.rec _ (not_le.mpr p ((8 : ℕ).le_add_left n))
+
+def Moore_fin4 : Moore ≃ fin 8 :=
+{ 
+  to_fun := Moore.to_fin8,
+  inv_fun := fin.toMoore,
+  left_inv := λ x, by {cases x; unfold Moore.to_fin8; refl},
+  right_inv := λ x, by {apply fin.toMoore.aux}
+}
 
 class neighborhood (α : Type) :=
   (size : nat)
@@ -93,41 +102,51 @@ class neighborhood (α : Type) :=
   (reflect : α → α)
 
 def vonNeumann.rotate_one : vonNeumann → vonNeumann
-  | vonNeumann.N := vonNeumann.E
-  | vonNeumann.E := vonNeumann.S
-  | vonNeumann.S := vonNeumann.W
-  | vonNeumann.W := vonNeumann.N
+  | N := E
+  | E := S
+  | S := W
+  | W := N
 
 def vonNeumann.reflect : vonNeumann → vonNeumann
-  | vonNeumann.E := vonNeumann.W
-  | vonNeumann.W := vonNeumann.E
+  | E := W
+  | W := E
   | x := x
 
 instance : neighborhood vonNeumann := 
   {
+    size := 4,
+    to_ix := vonNeumann_fin4,
     rotate_one := vonNeumann.rotate_one, 
     reflect := vonNeumann.reflect
   }
 
 def Moore.rotate_one : Moore → Moore
-  | Moore.N := Moore.NE
-  | Moore.NE := Moore.E
-  | Moore.E := Moore.SE
-  | Moore.SE := Moore.S
-  | Moore.S := Moore.SW
-  | Moore.SW := Moore.W
-  | Moore.W := Moore.NW
-  | Moore.NW := Moore.N
+  | NN := NE
+  | NE := EE
+  | EE := SE
+  | SE := SS
+  | SS := SW
+  | SW := WW
+  | WW := NW
+  | NW := NN
 
 
 def Moore.reflect : Moore → Moore
-  | Moore.NE := Moore.NW
-  | Moore.NW := Moore.NE
-  | Moore.E := Moore.W
-  | Moore.W := Moore.E
-  | Moore.SE := Moore.SW
-  | Moore.SW := Moore.SE
+  | NE := NW
+  | NW := NE
+  | EE := WW
+  | WW := EE
+  | SE := SW
+  | SW := SE
   | x := x
+
+instance : neighborhood Moore :=
+{ 
+  size := 8,
+  to_ix := Moore_fin4,
+  rotate_one := Moore.rotate_one,
+  reflect := Moore.reflect
+}
 
 inductive symmetries
   | none
@@ -139,24 +158,131 @@ inductive symmetries
   | reflect
   | permute
 
-structure var_line :=
+structure var_line (n : ℕ) :=
   (name : string)
-  (values : finset nat)
+  (values : finset (fin n))
 
 inductive value (n : nat)
-  | lit : fin n → value
   | var : string → value
+  | lit : fin n → value
 
-structure transition (nh : Type) (n : nat) : Type := 
-  (orig : value n)
-  (neighboorhood : nh → (value n))
-  (new : value n)
+def value.equiv_sum (n) : (string ⊕ fin n) ≃ value n :=
+  {
+    to_fun := sum.elim value.var value.lit,
+    inv_fun := λ v, value.cases_on v sum.inl sum.inr,
+    left_inv := λ x, by {simp, cases x; refl},
+    right_inv := λ x, by {simp, cases x; refl},
+  }
+
+instance subtype.encodable {α} [encodable α] (p : α → Prop) [decidable_pred p] : encodable (subtype p) := 
+{ 
+  encode := λ s, encodable.encode s.val,
+  decode := λ n, 
+    (do
+      (a : α) ← encodable.decode α n,
+      if h : p a
+        then some (⟨a, h⟩ : subtype p)
+        else none
+    ),
+
+  encodek := by {
+    intros,
+    obtain ⟨a, h⟩ := a,
+    simp,
+    rw subtype.encodable._match_1,
+    split_ifs, refl,
+  }
+}
+
+def char.equiv : subtype is_valid_char ≃ char := {
+  to_fun := λ ⟨x, p⟩, ⟨x, p⟩,
+  inv_fun := λ ⟨x, p⟩, ⟨x, p⟩,
+  left_inv := λ ⟨x, p⟩, by {simp, rw char.equiv._match_1, rw char.equiv._match_2},
+  right_inv := λ ⟨x, p⟩, by {simp, rw char.equiv._match_2, rw char.equiv._match_1},
+}
+
+instance : encodable char := encodable.of_equiv (subtype is_valid_char) char.equiv.symm
+
+def string_list : string ≃ list char := {
+  to_fun := string.to_list,
+  inv_fun := list.as_string,
+  left_inv := string.as_string_inv_to_list,
+  right_inv := list.to_list_inv_as_string
+}
+
+instance : encodable string := encodable.of_equiv (list char) string_list
+
+instance (n) : encodable (value n) := 
+  encodable.of_equiv (string ⊕ fin n) (value.equiv_sum n)
+.symm
+open value
+
+def linear_order.preimage {α β : Type} (f : α ↪ β) [lo : linear_order β] : linear_order α :=
+{
+  le := λ x y, f x ≤ f y,
+
+  le_refl := λ x, linear_order.le_refl (f x),
+
+  le_antisymm := λ (x y : α) x_y y_x, function.embedding.injective f (linear_order.le_antisymm (f x) (f y) x_y y_x),
+
+  le_trans := λ (x y z : α), linear_order.le_trans (f x) (f y) (f z),
+
+  le_total := λ (a b : α), linear_order.le_total (f a) (f b),
+
+  decidable_le := λ a b, if h : f a ≤ f b then is_true h else is_false h
+}
+
+instance {n} : linear_order (value n) := linear_order.preimage (encodable.encode' (value n))
+
+def transition (nh : Type) [nh_ : neighborhood nh] (num_states : nat) : Type := array (nh_.size + 2) (value num_states)
+
+def transition.orig {nh num_states} [nh_ : neighborhood nh] (arr : transition nh num_states) : value num_states := arr.read 0
+def transition.neihborhood {nh num_states} [nh_ : neighborhood nh] (arr : transition nh num_states) (ix : nh) : value num_states :=
+  arr.read (neighborhood.to_ix ix)
+
+instance (nh : Type) [nh_ : neighborhood nh] (n : nat) : encodable (transition nh n) :=
+  encodable.of_equiv (array (nh_.size + 2) (value n)) (equiv.refl _)
+
+def transition.le {nh : Type} [nh_ : neighborhood nh] {n : nat} : (transition nh n) → (transition nh n) → Prop :=
+  (encodable.encode' (transition nh n)) ⁻¹'o (has_le.le : ℕ → ℕ → Prop)
+
+@[simp]
+lemma transition.le.def {nh : Type} [nh_ : neighborhood nh] {n : nat} (a b : transition nh n) :
+  a.le b = ((encodable.encode' (transition nh n)) ⁻¹'o (has_le.le : ℕ → ℕ → Prop)) a b := rfl
+
+instance (nh : Type) [nh_ : neighborhood nh] (n : nat) : linear_order (transition nh n)  := 
+  { 
+    le := transition.le,
+    le_refl := λ a, by {unfold1 has_le.le, simp},
+    le_trans := λ x y z, by {simp, apply le_trans},
+    
+    le_antisymm := λ x y, 
+    by {
+      unfold_projs, simp,
+      intros x_y y_x, 
+      apply function.embedding.injective (encodable.encode' _), 
+      exact le_antisymm x_y y_x
+    },
+
+    le_total :=  λ x y, by {unfold_projs, simp, apply le_total},
+    decidable_le := λ x y,
+      if h : encodable.encode' _ x ≤ encodable.encode' _ y
+        then is_true h
+        else is_false h,
+    decidable_eq := λ x y,
+    if h : encodable.encode' _ x = encodable.encode' _ y
+        then is_true (function.embedding.injective (encodable.encode' _) h)
+        else is_false (λ x_eq_y : x = y, by {apply h, congr, exact x_eq_y}),
+    decidable_lt := λ x y,
+    if h : encodable.encode' _ x < encodable.encode' _ y
+        then is_true h
+        else is_false h,
+  }
 
 infix `~>`:40 := λ α β, finmap (λ _ : α, β)
 
-structure rule_table :=
+structure rule_table (nh : Type) [h : neighborhood nh] :=
   (n_states : nat)
-  (nh : Type)
   (symmetries: symmetries)
   (vars : string ~> (fin n_states))
   (transitions : rbtree (transition nh n_states))
